Working functions: setup_pool, async, await

share/steel/examples/pulse/parallel/DomainsPoolAlive.fsti
@@ -5,9 +5,364 @@ module Lock = Pulse.Lib.SpinLock
 module HR = Pulse.Lib.HigherReference
 module M = Pulse.Lib.GhostMonotonicHigherReference
 
-let thunk a p
-  = unit -> stt unit (pts_to p #one_half None) (fun () ->
-    exists* v. pts_to p #one_half (Some v))
+module GR = Pulse.Lib.GhostReference
+
+open SingleGhostTask
+open GhostTaskQueue
+
+(* Pool: ghost_mono_ref, counter, task queue, lock, invariant... *)
+
+let task_queue: Type0 = list task
+
+(* also ghost queue? *)
+val mono_queue_ref: Type0
+val mono_queue: Type0 (* not 0? *)
+
+let link (l: mono_list) (q: task_queue) (c: int): prop
+= (count_ongoing l == c /\ get_actual_queue l == q)
+
+
+let if_then_else (b: bool) (thn: vprop) (els: vprop): vprop
+= if b then thn else els
+
+let lock_thn (l: mono_list) q c: vprop
+= (exists* vq vc. pts_to q vq ** pts_to c vc ** pure (link l vq vc))
+
+let lock_els l status_pool: vprop
+= (pure (link l [] 0) ** (exists* f1. pts_to status_pool #f1 false))
+(* maybe we'll need some permission to the ghost_mono_ref? maybe not *)
+
+
+let lock_pool
+  (status_pool: ref bool)
+  (q: ref task_queue)
+  (c: ref int)
+  (r: ghost_mono_ref)
+: vprop
+= (exists* sp l. pts_to status_pool #one_half sp ** M.pts_to r one_half l
+  ** (if_then_else sp (lock_thn l q c) (lock_els l status_pool)))
+
+let pool = (status_pool: ref bool
+  & q: ref task_queue
+  & c: ref int
+  & ri: (r:ghost_mono_ref & inv (inv_ghost_queue r))
+  & Lock.lock (lock_pool status_pool q c ri._1))
+
+let mk_pool (status_pool: ref bool) (q: ref task_queue)
+  (c: ref int) (ri: (r:ghost_mono_ref & inv (inv_ghost_queue r)))
+  (lock: Lock.lock (lock_pool status_pool q c ri._1)): pool
+= (| status_pool, q, c, ri, lock |)
+
+let pool_alive (f: perm) (p: pool): vprop // f/2 permission to the ghost bool ref, true
+= pts_to p._1 #(half_perm f) true
+
+
+let locked_pool (p: pool): vprop =
+  lock_pool p._1 p._2 p._3 p._4._1
+
+```pulse
+ghost fn elim_if_then
+(b: bool) (thn: vprop) (els: vprop)
+requires if_then_else b thn els ** pure b
+ensures thn
+{
+  rewrite if_then_else b thn els as thn
+}
+```
+
+
+
+//#push-options "--print_implicits"
+```pulse
+ghost fn
+unfold_lock_pool_alive (#f: perm) (pl: pool)
+requires pool_alive f pl ** locked_pool pl
+//requires lock_pool pl._1 pl._2 pl._3 pl._4._1 ** pool_alive f pl
+ensures pool_alive f pl ** (exists* sp l. pts_to pl._1 #one_half sp ** M.pts_to pl._4._1 one_half l **
+  (exists* vq vc. pts_to pl._2 vq ** pts_to pl._3 vc ** pure (link l vq vc)))
+{
+  unfold locked_pool pl;
+  unfold lock_pool;
+  unfold pool_alive f pl;
+  with sp gq. assert (pts_to pl._1 #one_half sp ** M.pts_to pl._4._1 one_half gq);
+  pts_to_injective_eq pl._1;
+  fold pool_alive f pl;
+  elim_if_then _ _ _;
+  unfold lock_thn; //_ pl._2 pl._3;
+  ()
+}
+```
+
+```pulse
+ghost fn
+fold_lock_pool_alive (#f: perm) (pl: pool)
+requires pool_alive f pl ** (exists* sp l. pts_to pl._1 #one_half sp ** M.pts_to pl._4._1 one_half l **
+  (exists* vq vc. pts_to pl._2 vq ** pts_to pl._3 vc ** pure (link l vq vc)))
+ensures pool_alive f pl ** locked_pool pl
+//requires lock_pool pl._1 pl._2 pl._3 pl._4._1 ** pool_alive f pl
+{
+  admit()
+  (*
+  unfold locked_pool pl;
+  unfold lock_pool;
+  unfold pool_alive f pl;
+  with sp gq. assert (pts_to pl._1 #one_half sp ** M.pts_to pl._4._1 one_half gq);
+  pts_to_injective_eq pl._1;
+  fold pool_alive f pl;
+  elim_if_then _ _ _;
+  unfold lock_thn; //_ pl._2 pl._3;
+  ()
+  *)
+}
+```
+(*
+TODO: Actually launch workers...
+*)
+```pulse
+fn setup_pool (n: int{n >= 1})
+  requires emp
+  returns pl: pool
+  ensures pool_alive full_perm pl
+{
+  let ri: (r: ghost_mono_ref & inv (inv_ghost_queue r)) = create_ghost_queue ();
+
+  let status_pool: ref bool = alloc true;
+  share2 status_pool;
+
+  let q: ref task_queue = alloc #task_queue [];
+  let c: ref int = alloc 0;
+
+  assert (pts_to q [] ** pts_to c 0 ** pure (link [] [] 0));
+  assert (exists* vq vc. pts_to q vq ** pts_to c vc ** pure (link [] vq vc));
+  fold lock_thn [] q c;
+  fold (if_then_else true (lock_thn [] q c) (lock_els [] status_pool));
+
+  fold (lock_pool status_pool q c ri._1);
+  let lock = Lock.new_lock (lock_pool status_pool q c ri._1);
+
+  let pl: pool = mk_pool status_pool q c ri lock;
+  rewrite each status_pool as pl._1;
+  fold pool_alive full_perm pl;
+  pl
+}
+```
+
+(*
+probably this lock needs to be in the task queue?
+*)
+
+type handler (pl: pool) (post: vprop) =
+  t:task & (pos:nat) & certificate pl._4._1 t pos //& Lock.lock (lock_task t)//(exists* v. pts_to t._4 #one_half v)
+
+let mk_handler_pure (pl: pool) (post: vprop) (t: task) (pos: nat) (certif: certificate pl._4._1 t pos)
+  //(lock: Lock.lock (lock_task t))
+  : handler pl post
+= (| t, pos, certif |)
+
+```pulse
+fn mk_handler
+(pl: pool) (post: vprop) (t: task) 
+(res: (pos:nat & certificate pl._4._1 t pos))
+//(pos: nat) (certif: certificate pl._4._1 t pos)
+requires GR.pts_to t._5 #one_half false
+returns h: handler pl post
+ensures GR.pts_to h._1._5 #one_half false
+{
+  //fold lock_task t;
+  //let lock = Lock.new_lock (lock_task t);
+  let h: handler pl post = mk_handler_pure pl post t res._1 res._2;
+  rewrite each t as h._1;
+  h
+}
+```
+  
+  //(lock: Lock.lock (exists* v. pts_to t._4 #one_half v)): handler pl post
+
+(*
+      GR.pts_to (Mkdtuple5?._5 t) (reveal (hide false)) ** 
+      pts_to (Mkdtuple5?._4 t) (reveal (hide false)) ** 
+    *)
+
+(*
+TODO:
+ASSUMING!
+*)
+(*
+val read_ghost_mono_ref (#a:Type) (#p:Preorder.preorder a) (#f: perm)
+    (r:M.ref a p)
+  : stt_atomic a #Unobservable emp_inames
+  (exists* v. M.pts_to r f v) (fun vv -> M.pts_to r f vv)
+  (* How wrong is this? *)
+  *)
+val read_ghost_mono_ref (#a:Type) (#p: Preorder.preorder a) (r:M.ref a p) (#n:erased a) (#p:perm)
+  : stt a
+        (M.pts_to r p n)
+        (fun x -> M.pts_to r p n ** pure (reveal n == x))
+
+let enqueue_add_task_get_actual (l: mono_list) (t: task) (vq: task_queue) (vc: int):
+  Lemma (requires link l vq vc)
+  (ensures link (enqueue_todo l t)._1 (t::vq) vc)
+= ()
+
+```pulse
+ghost fn pulse_enqueue_add_task_get_actual (l: mono_list) (t: task) (vq: task_queue) (vc: int)
+requires pure (link l vq vc)
+ensures pure (link (enqueue_todo l t)._1 (t::vq) vc)
+{
+  ()
+}
+```
+
+
+
+val assume_prop (p: prop):
+stt unit emp (fun () -> pure p)
+
+#push-options "--print_implicits"
+```pulse
+fn async #pre #post #f (pl: pool) (ta: (unit -> stt unit pre (fun () -> post)))
+  requires pool_alive f pl ** pre
+  returns h: handler pl post
+  // returns pr: promise pl unit post, or handler
+  ensures pool_alive f pl ** GR.pts_to h._1._5 #one_half false
+  // ** pledge (task_done pr) post
+{
+  let ti: (t: task & inv (guarded_inv t._2 post)) = create_task ta;
+  let t = ti._1;
+  let itask: inv (guarded_inv t._2 post) = ti._2;
+
+  let status_pool: ref bool = pl._1;
+  let q: ref task_queue = pl._2;
+  let c: ref int = pl._3;
+  let r: ghost_mono_ref = pl._4._1;
+  let i: inv (inv_ghost_queue r) = pl._4._2;
+  let lock = pl._5;
+
+  Lock.acquire pl._5;
+  //show_proof_state;
+  rewrite (lock_pool (Mkdtuple5?._1 pl) (Mkdtuple5?._2 pl) (Mkdtuple5?._3 pl) (Mkdtuple2?._1 (Mkdtuple5?._4 pl)))
+    as locked_pool pl;//(lock_pool status_pool q c r);
+  unfold_lock_pool_alive pl;
+
+  rewrite each pl._1 as status_pool;
+  rewrite each pl._2 as q;
+  rewrite each pl._3 as c;
+  rewrite each pl._4._1 as r;
+  rewrite each pl._4._2 as i;
+  rewrite each pl._5 as lock;
+  rewrite each ti._1 as t;
+
+  //with ll. assert (M.pts_to r one_half ll);
+  let l: mono_list = read_ghost_mono_ref r;
+  let ll: mono_list = (enqueue_todo l t)._1;
+  with vq vc. assert (pts_to q vq ** pts_to c vc);
+  let vq_: task_queue = !q;
+  let vq': task_queue = Prims.Cons #task t vq_;
+  assert pure (link l vq vc);
+  assert pure (link ll vq' vc);
+
+  rewrite each ti._1 as t;
+  //share2 t._4._1;
+  assert GR.pts_to t._5 #full_perm false;
+  GR.share2 t._5;
+  assert GR.pts_to t._5 #one_half false ** GR.pts_to t._5 #one_half false;
+  let res: (pos:nat & certificate r t pos) = add_todo_task_to_queue r i t l;
+  //assert M.pts_to r one_half (enqueue_todo l t)._1;
+
+  assert pts_to q (reveal vq);
+  q := vq'; //(enqueue_todo l t)._1;
+  assert pure (link ll vq' vc);
+  assert pool_alive f pl;
+  with sp. assert pts_to status_pool #one_half sp ** M.pts_to r one_half ll;
+
+  assert pool_alive f pl;
+  rewrite each status_pool as pl._1;
+  rewrite each q as pl._2;
+  rewrite each c as pl._3;
+  rewrite each r as pl._4._1;
+  assert (exists* sp l. pts_to pl._1 #one_half sp ** M.pts_to pl._4._1 one_half l **
+  (exists* vq vc. pts_to pl._2 vq ** pts_to pl._3 vc ** pure (link l vq vc)));
+  fold_lock_pool_alive pl;
+  rewrite (locked_pool pl) as lock_pool pl._1 pl._2 pl._3 pl._4._1;
+  Lock.release pl._5;
+  let h: handler pl post = mk_handler pl post t res;
+  h
+}
+```
+
+```pulse
+ghost fn get_task_done (t: task) (f: perm)
+requires pts_to t._4._1 #f true
+ensures task_done t
+{
+  fold task_done t
+}
+```
+
+```pulse
+ghost fn close_lock_task (bdone: ref bool) (f: perm) (v: bool)
+requires pts_to bdone #f v ** pure (if not v then f == one_half else true)
+ensures lock_task bdone
+{
+  admit()
+}
+```
+
+(*
+pool_alive is currently not necessary, because we never deallocate the reference where we say whether we're done...
+*)
+#pop-options
+```pulse
+fn await (#pl: pool) (#post: vprop) (h: handler pl post)
+  requires pool_alive f pl
+  ensures pool_alive f pl ** task_done h._1
+{
+  let mut task_is_done = false;
+  rewrite emp as (if false then task_done h._1 else emp);
+  let bdone: ref bool = h._1._4._1;
+  let lock: Lock.lock (lock_task bdone) = h._1._4._2;
+  while (let d = !task_is_done; not d)
+    invariant b. (exists* d. pts_to task_is_done d ** pure (b == not d) ** (if d then task_done h._1 else emp)
+    //** pure (bdone == h._1._4._1) 
+    )
+  {
+    with d. assert pts_to task_is_done d;
+    Lock.acquire lock;
+    rewrite lock_task bdone
+      as (exists* v f. pts_to bdone #f v ** pure (if not v then f == one_half else true));
+    with v f. assert pts_to bdone #f v ** pure (if not v then f == one_half else true);
+    let vdone: bool = !bdone;
+    task_is_done := vdone;
+    rewrite (match reveal d <: bool with | true -> task_done (Mkdtuple3?._1 h) | _ -> emp) as emp;
+    if (vdone) {
+      share bdone;
+      assert pure (bdone == h._1._4._1);
+      rewrite (pts_to bdone #(half_perm f) v) as pts_to h._1._4._1 #(half_perm f) true;
+      assert pts_to h._1._4._1 #(half_perm f) true;
+      get_task_done h._1 (half_perm f);
+      rewrite task_done h._1 as (if true then task_done h._1 else emp);
+      close_lock_task bdone (half_perm f) true;
+      Lock.release h._1._4._2;
+      assert pts_to task_is_done true;
+      assert (pts_to task_is_done true ** (if true then task_done h._1 else emp));
+      ()
+    }
+    else {
+      rewrite emp as (if false then task_done h._1 else emp);
+      close_lock_task bdone f false;
+      Lock.release h._1._4._2;
+      ()
+    }
+  };
+  with d. assert pts_to task_is_done d;
+  assert (if d then task_done h._1 else emp) ** pure (false = not d);
+  elim_if_then d _ emp;
+  //rewrite (if d then task_done h._1 else emp) as task_done h._1;
+  ()
+}
+```
+
+
 
 (*
 + there's an invariant somewhere that proves post of Some x
@@ -16,39 +371,7 @@ let thunk a p
 (* where are stored the invariant? *)
 (* in the certificate... *)
 
-let task_elem = (
-  a: Type0 // return type of the computation
-  & p: ref (option a) // the reference where we put the result of the computation
-  & thunk a p // the computation
-)
 
-let task_queue: Type u#1 = list task_elem
-// depends negatively on pool
-
-(* also ghost queue? *)
-val mono_queue_ref: Type0
-val mono_queue: Type0 (* not 0? *)
-
-val pts_to_mono_queue
-  (ghost_queue: mono_queue_ref) (f: perm) (value: mono_queue): vprop
-
-val gather2_mono_queue (r:mono_queue_ref) (#x0 #x1:erased mono_queue)
-  : stt_ghost unit
-      (pts_to_mono_queue r one_half x0 ** pts_to_mono_queue r one_half x1)
-      (fun _ -> pts_to_mono_queue r full_perm x0 ** pure (x0 == x1))
-
-(* Share/gather specialized to half permission *)
-val share2_mono_queue (r:mono_queue_ref) (#v:erased mono_queue)
-  : stt_ghost unit
-      (pts_to_mono_queue r full_perm v)
-      (fun _ -> pts_to_mono_queue r one_half v ** pts_to_mono_queue r one_half v)
-
-
-
-val link (gq: mono_queue) (q: task_queue) (c: int): prop
-(*
-  count_ongoing l = c /\ get_actual_queue l == q
-*)
 (*
 let small_inv (r: erased (ghost_mono_ref task_elem)) (q: list task_elem) (c: int): vprop 
 = exists_ (fun l -> pts_to_ghost_queue_half r l **
@@ -64,19 +387,6 @@ could be:
 
 *)
 
-let if_then_else (b: bool) (thn: vprop) (els: vprop): vprop
-= if b then thn else els
-
-```pulse
-ghost fn elim_if_then
-(b: bool) (thn: vprop) (els: vprop)
-requires if_then_else b thn els ** pure b
-ensures thn
-{
-  rewrite if_then_else b thn els as thn
-}
-```
-
 ```pulse
 ghost fn intro_if_then
 (b: bool) (thn: vprop) (els: vprop)
@@ -87,35 +397,6 @@ ensures if_then_else b thn els
 }
 ```
 
-let lock_thn gq ghost_queue queue counter: vprop
-= (pts_to_mono_queue ghost_queue one_half gq ** (exists* q c. HR.pts_to queue q ** pts_to counter c ** pure (link gq q c)))
-
-let lock_els gq status_pool ghost_queue: vprop
-= (pure (link gq [] 0) ** (exists* f1 f2. pts_to status_pool #f1 false ** pts_to_mono_queue ghost_queue f2 gq))
-
-
-let lock_pool
-  (status_pool: ref bool)
-  (queue: HR.ref task_queue)
-  (counter: ref int)
-  (ghost_queue: mono_queue_ref)
-: vprop
-= (exists* sp gq. pts_to status_pool #one_half sp ** pts_to_mono_queue ghost_queue one_half gq
-  ** (if_then_else sp (lock_thn gq ghost_queue queue counter) (lock_els gq status_pool ghost_queue)))
-
-
-let pool = (status_pool: ref bool
-  & queue: HR.ref task_queue
-  & counter: ref int
-  & ghost_queue: mono_queue_ref
-  & Lock.lock (lock_pool status_pool queue counter ghost_queue))
-
-let locked_pool (p: pool): vprop =
-  lock_pool p._1 p._2 p._3 p._4
-
-
-let pool_alive (f: perm) (p: pool): vprop // f/2 permission to the ghost bool ref, true
-= pts_to p._1 #(half_perm f) true
 
 ```pulse
 ghost fn open_lock_pool_alive
